doASP no longer admitted

src/Cvm_Impl.v
@@ -10,32 +10,32 @@ Require Import List.
 Import ListNotations.
 
 (** Monadic CVM implementation (top-level) *)
-Fixpoint build_cvm (t:Core_Term): CVM unit :=
+Fixpoint build_cvm (t:Core_Term) (ac : AM_Config) : CVM unit :=
   match t with
   | aspc a =>
-      e <- do_prim a ;;
+      e <- do_prim a ac ;;
       put_ev e
   | attc q t' =>
     e <- get_ev ;;
     e' <- doRemote t' q e ;;
     put_ev e'
   | lseqc t1 t2 =>
-      build_cvm t1 ;;
-      build_cvm t2
+      build_cvm t1 ac ;;
+      build_cvm t2 ac
   | bseqc t1 t2 =>
     split_ev ;;
     e <- get_ev ;;
-    build_cvm t1 ;;
+    build_cvm t1 ac ;;
     e1r <- get_ev ;;
     put_ev e ;;
-    build_cvm t2 ;;
+    build_cvm t2 ac ;;
     e2r <- get_ev ;;
     join_seq e1r e2r
   | bparc loc t1 t2 =>
     split_ev ;;
     e <- get_ev ;;
     start_par_thread loc t2 e ;;
-    build_cvm t1 ;;
+    build_cvm t1 ac ;;
     e1r <- get_ev ;;
     e2r <- wait_par_thread loc t2 e ;;
     join_seq e1r e2r
